clc

coq/theories/clc.v
@@ -385,8 +385,8 @@ Qed.
 Inductive term : Type :=
 | Var   (x : var)
 | Sort  (s : sort) (l : option nat)
-| Prod  (A : term) (B : {bind term}) (s t : sort)
-| Lolli (A : term) (B : {bind term}) (s t : sort)
+| Prod  (A : term) (B : {bind term}) (s : sort)
+| Lolli (A : term) (B : {bind term}) (s : sort)
 | Lam   (n : {bind term})
 | App   (m n : term).
 
@@ -396,11 +396,11 @@ Instance Subst_term : Subst term. derive. Defined.
 Instance substLemmas_term : SubstLemmas term. derive. Qed.
 
 Inductive value : term -> Prop :=
-| value_sort srt l    : value (Sort srt l)
-| value_var x         : value (Var x)
-| value_prod A B s t  : value (Prod A B s t)
-| value_lolli A B s t : value (Lolli A B s t)
-| value_lam n         : value (Lam n).
+| value_sort srt l  : value (Sort srt l)
+| value_var x       : value (Var x)
+| value_prod A B s  : value (Prod A B s)
+| value_lolli A B s : value (Lolli A B s)
+| value_lam n       : value (Lam n).
 
 Reserved Notation "m ~> n" (at level 30).
 Inductive step : term -> term -> Prop :=
@@ -409,18 +409,18 @@ Inductive step : term -> term -> Prop :=
 | step_lam m m' :
   m ~> m' ->
   Lam m ~> Lam m'
-| step_prodL A A' B s t :
+| step_prodL A A' B s :
   A ~> A' ->
-  Prod A B s t ~> Prod A' B s t
-| step_prodR A B B' s t :
+  Prod A B s ~> Prod A' B s
+| step_prodR A B B' s :
   B ~> B' ->
-  Prod A B s t ~> Prod A B' s t
-| step_lolliL A A' B s t :
+  Prod A B s ~> Prod A B' s
+| step_lolliL A A' B s :
   A ~> A' ->
-  Lolli A B s t ~> Lolli A' B s t
-| step_lolliR A B B' s t :
+  Lolli A B s ~> Lolli A' B s
+| step_lolliR A B B' s :
   B ~> B' ->
-  Lolli A B s t ~> Lolli A B' s t
+  Lolli A B s ~> Lolli A B' s
 | step_appL m m' n :
   m ~> m' ->
   App m n ~> App m' n
@@ -445,16 +445,16 @@ Inductive pstep : term -> term -> Prop :=
   pstep m m' ->
   pstep n n' ->
   pstep (App (Lam m) n) (m'.[n'/])
-| pstep_prod A A' s B B' t :
+| pstep_prod A A' s B B' :
   pstep A A' ->
   pstep B B' ->
-  pstep (Prod A B s t) 
-        (Prod A' B' s t)
-| pstep_lolli A A' s B B' t :
+  pstep (Prod A B s) 
+        (Prod A' B' s)
+| pstep_lolli A A' s B B' :
   pstep A A' ->
   pstep B B' ->
-  pstep (Lolli A B s t) 
-        (Lolli A' B' s t).
+  pstep (Lolli A B s) 
+        (Lolli A' B' s).
 
 Notation red := (star step).
 Notation "m ~>* n" := (red m n) (at level 30).
@@ -482,20 +482,20 @@ Qed.
 Lemma red_lam s1 s2 : s1 ~>* s2 -> Lam s1 ~>* Lam s2.
 Proof. apply: star_hom => x y. exact: step_lam. Qed.
 
-Lemma red_prod A1 A2 B1 B2 s t :
-  A1 ~>* A2 -> B1 ~>* B2 -> Prod A1 B1 s t ~>* Prod A2 B2 s t.
+Lemma red_prod A1 A2 B1 B2 s :
+  A1 ~>* A2 -> B1 ~>* B2 -> Prod A1 B1 s ~>* Prod A2 B2 s.
 Proof.
-  move=> A B. apply: (star_trans (Prod A2 B1 s t)).
-  - apply: (star_hom (((Prod^~ B1)^~ s)^~ t)) A => x y. exact: step_prodL.
-  - apply: (star_hom (((Prod A2)^~ s)^~ t)) B => x y. exact: step_prodR.
+  move=> A B. apply: (star_trans (Prod A2 B1 s)).
+  - apply: (star_hom ((Prod^~ B1)^~ s)) A => x y. exact: step_prodL.
+  - apply: (star_hom ((Prod A2)^~ s)) B => x y. exact: step_prodR.
 Qed.
 
-Lemma red_lolli A1 A2 B1 B2 s t :
-  A1 ~>* A2 -> B1 ~>* B2 -> Lolli A1 B1 s t ~>* Lolli A2 B2 s t.
+Lemma red_lolli A1 A2 B1 B2 s :
+  A1 ~>* A2 -> B1 ~>* B2 -> Lolli A1 B1 s ~>* Lolli A2 B2 s.
 Proof.
-  move=> A B. apply: (star_trans (Lolli A2 B1 s t)).
-  - apply: (star_hom (((Lolli^~ B1)^~ s)^~ t)) A => x y. exact: step_lolliL.
-  - apply: (star_hom (((Lolli A2)^~ s)^~ t)) B => x y. exact: step_lolliR.
+  move=> A B. apply: (star_trans (Lolli A2 B1 s)).
+  - apply: (star_hom ((Lolli^~ B1)^~ s)) A => x y. exact: step_lolliL.
+  - apply: (star_hom ((Lolli A2)^~ s)) B => x y. exact: step_lolliR.
 Qed.
 
 Lemma red_subst m n : 
@@ -523,23 +523,23 @@ Definition sconv (σ τ : var -> term) :=
 Lemma conv_lam s1 s2 : s1 === s2 -> Lam s1 === Lam s2.
 Proof. apply: conv_hom => x y. exact: step_lam. Qed.
 
-Lemma conv_prod A A' s B B' t :
-  A === A' -> B === B' -> Prod A B s t === Prod A' B' s t.
+Lemma conv_prod A A' s B B' :
+  A === A' -> B === B' -> Prod A B s === Prod A' B' s.
 Proof.
-  move=> conv1 conv2. apply: (conv_trans (Prod A' B s t)).
-  - apply: (conv_hom (((Prod^~ B)^~ s)^~ t)) conv1 => x y ps.
+  move=> conv1 conv2. apply: (conv_trans (Prod A' B s)).
+  - apply: (conv_hom ((Prod^~ B)^~ s)) conv1 => x y ps.
     constructor; eauto.
-  - apply: (conv_hom (((Prod A')^~ s)^~ t)) conv2 => x y ps.
+  - apply: (conv_hom ((Prod A')^~ s)) conv2 => x y ps.
     constructor; eauto.
 Qed.
 
-Lemma conv_lolli A A' s B B' t :
-  A === A' -> B === B' -> Lolli A B s t === Lolli A' B' s t.
+Lemma conv_lolli A A' s B B' :
+  A === A' -> B === B' -> Lolli A B s === Lolli A' B' s.
 Proof.
-  move=> conv1 conv2. apply: (conv_trans (Lolli A' B s t)).
-  - apply: (conv_hom (((Lolli^~ B)^~ s)^~ t)) conv1 => x y ps.
+  move=> conv1 conv2. apply: (conv_trans (Lolli A' B s)).
+  - apply: (conv_hom ((Lolli^~ B)^~ s)) conv1 => x y ps.
     constructor; eauto.
-  - apply: (conv_hom (((Lolli A')^~ s)^~ t)) conv2 => x y ps.
+  - apply: (conv_hom ((Lolli A')^~ s)) conv2 => x y ps.
     constructor; eauto.
 Qed.
 
@@ -697,10 +697,10 @@ Proof with eauto using pstep.
       exists (x0.[x/]). split.
       * apply pstep_compat_beta...
       * apply pstep_compat_beta...
-  - inv H1. apply (IHpstep1) in H7. apply (IHpstep2) in H8.
-    first_order. exists (Prod x0 x s t)...
-  - inv H1. apply (IHpstep1) in H7. apply (IHpstep2) in H8.
-    first_order. exists (Lolli x0 x s t)...
+  - inv H1. apply (IHpstep1) in H6. apply (IHpstep2) in H7.
+    first_order. exists (Prod x0 x s)...
+  - inv H1. apply (IHpstep1) in H6. apply (IHpstep2) in H7.
+    first_order. exists (Lolli x0 x s)...
 Qed.
 
 Lemma strip m m1 m2 :
@@ -754,16 +754,16 @@ Proof.
   induction v; asimpl; try discriminate; eauto.
 Qed.
 
-Lemma prod_ren_inv A B s t v xi :
-  Prod A B s t = v.[ren xi] -> 
-  exists A B s t, v = Prod A B s t.
+Lemma prod_ren_inv A B s v xi :
+  Prod A B s = v.[ren xi] -> 
+  exists A B s, v = Prod A B s.
 Proof.
   induction v; asimpl; try discriminate; eauto 6.
 Qed.
 
-Lemma lolli_ren_inv A B s t v xi :
-  Lolli A B s t = v.[ren xi] -> 
-  exists A B s t, v = Lolli A B s t.
+Lemma lolli_ren_inv A B s v xi :
+  Lolli A B s = v.[ren xi] -> 
+  exists A B s, v = Lolli A B s.
 Proof.
   induction v; asimpl; try discriminate; eauto 6.
 Qed.
@@ -799,12 +799,12 @@ Proof.
   inv H0; eauto.
 Qed.
 
-Lemma red_prod_inv A B s t x :
-  red (Prod A B s t) x -> 
+Lemma red_prod_inv A B s x :
+  red (Prod A B s) x -> 
   exists A' B',
     red A A' /\
     red B B' /\
-    x = Prod A' B' s t.
+    x = Prod A' B' s.
 Proof.
   induction 1.
   - exists A.
@@ -824,12 +824,12 @@ Proof.
       econstructor; eauto.
 Qed.
 
-Lemma red_lolli_inv A B s t x :
-  red (Lolli A B s t) x -> 
+Lemma red_lolli_inv A B s x :
+  red (Lolli A B s) x -> 
   exists A' B',
     red A A' /\
     red B B' /\
-    x = Lolli A' B' s t.
+    x = Lolli A' B' s.
 Proof.
   induction 1.
   - exists A.
@@ -882,9 +882,9 @@ Proof.
   first_order; subst; inv H1; eauto.
 Qed.
 
-Lemma prod_inj A A' B B' s s' t t' :
-  Prod A B s t === Prod A' B' s' t' ->
-  A === A' /\ B === B' /\ s = s' /\ t = t'.
+Lemma prod_inj A A' B B' s s' :
+  Prod A B s === Prod A' B' s' ->
+  A === A' /\ B === B' /\ s = s'.
 Proof.
   intros.
   apply church_rosser in H.
@@ -895,12 +895,11 @@ Proof.
   inv H2; eauto using join_conv.
   inv H2; eauto using join_conv.
   inv H2; eauto.
-  inv H2; eauto.
 Qed.
 
-Lemma lolli_inj A A' B B' s s' t t' :
-  Lolli A B s t === Lolli A' B' s' t' ->
-  A === A' /\ B === B' /\ s = s' /\ t = t'.
+Lemma lolli_inj A A' B B' s s' :
+  Lolli A B s === Lolli A' B' s' ->
+  A === A' /\ B === B' /\ s = s'.
 Proof.
   intros.
   apply church_rosser in H.
@@ -910,7 +909,6 @@ Proof.
   first_order; subst.
   inv H2; eauto using join_conv.
   inv H2; eauto using join_conv.
-  inv H2; eauto.
   inv H2; eauto.
 Qed.
 
@@ -958,12 +956,12 @@ Inductive sub1 : term -> term -> Prop :=
 | sub1_sort s l1 l2 : 
   l1 <= l2 -> 
   sub1 (s @ l1) (s @ l2)
-| sub1_prod A B1 B2 s t : 
+| sub1_prod A B1 B2 s : 
   sub1 B1 B2 -> 
-  sub1 (Prod A B1 s t) (Prod A B2 s t)
-| sub1_lolli A B1 B2 s t : 
+  sub1 (Prod A B1 s) (Prod A B2 s)
+| sub1_lolli A B1 B2 s : 
   sub1 B1 B2 -> 
-  sub1 (Lolli A B1 s t) (Lolli A B2 s t).
+  sub1 (Lolli A B1 s) (Lolli A B2 s).
 
 CoInductive sub (A B : term) : Prop :=
 | SubI A' B' : 
@@ -994,8 +992,8 @@ Proof with eauto 6 using sub1, sub1_sub, sub1_conv, conv_sub1.
     [ A C D 
     | s l C D conv sb
     | s l1 l2 leq C D conv sb
-    | A B1 B2 s t sb1 ih C D conv sb2
-    | A B1 B2 s t sb1 ih C D conv sb2 ]...
+    | A B1 B2 s sb1 ih C D conv sb2
+    | A B1 B2 s sb1 ih C D conv sb2 ]...
   - inv sb; try (exfalso; solve_conv)...
     move: conv => /sort_inj [->[eq]].
     apply: sub_prop.
@@ -1004,14 +1002,14 @@ Proof with eauto 6 using sub1, sub1_sub, sub1_conv, conv_sub1.
     apply: sub_sort. subst.
     exact: leq_trans leq _.
   - inv sb2; try (exfalso; solve_conv)...
-    move: conv => /prod_inj[conv1 [conv2 [->->]]].
+    move: conv => /prod_inj[conv1 [conv2 ->]].
     move: (ih _ _ conv2 H) => {ih} sub. inv sub.
     eapply SubI. 
     eapply sub1_prod... 
     eapply conv_prod... 
     exact: conv_prod.
   - inv sb2; try (exfalso; solve_conv)...
-    move: conv => /lolli_inj[conv1 [conv2 [->->]]].
+    move: conv => /lolli_inj[conv1 [conv2 ->]].
     move: (ih _ _ conv2 H) => {ih} sub. inv sub.
     eapply SubI. 
     eapply sub1_lolli... 
@@ -1055,40 +1053,40 @@ Proof.
   - move=> *. exfalso; solve_conv.
 Qed.
 
-Lemma sub_prod_inv A1 A2 s1 s2 B1 B2 t1 t2 :
-  Prod A1 B1 s1 t1 <: Prod A2 B2 s2 t2 -> 
-  A1 === A2 /\ B1 <: B2 /\ s1 = s2 /\ t1 = t2.
+Lemma sub_prod_inv A1 A2 s1 s2 B1 B2 :
+  Prod A1 B1 s1 <: Prod A2 B2 s2 -> 
+  A1 === A2 /\ B1 <: B2 /\ s1 = s2.
 Proof.
   move=> [A' B' []].
   - move=> C c1 c2. 
-    have{c1 c2}/prod_inj[c1 [c2 [->->]]]: 
-      Prod A1 B1 s1 t1 === Prod A2 B2 s2 t2.
+    have{c1 c2}/prod_inj[c1 [c2 ->]]: 
+      Prod A1 B1 s1 === Prod A2 B2 s2.
      exact: conv_trans c2.
     firstorder=>//. exact: conv_sub.
   - move=> *. exfalso; solve_conv.
   - move=> *. exfalso; solve_conv.
-  - move=> A B0 B3 s t sb /prod_inj[c1 [c2 [<-<-]]]. 
-    move=> /prod_inj[c3 [c4 [->->]]]. 
+  - move=> A B0 B3 s sb /prod_inj[c1 [c2 <-]]. 
+    move=> /prod_inj[c3 [c4 ->]]. 
     firstorder.
     exact: conv_trans c3. exact: SubI sb c2 c4.
   - move=> *. exfalso; solve_conv.
 Qed.
 
-Lemma sub_lolli_inv A1 A2 s1 s2 B1 B2 t1 t2 :
-  Lolli A1 B1 s1 t1 <: Lolli A2 B2 s2 t2 -> 
-  A1 === A2 /\ B1 <: B2 /\ s1 = s2 /\ t1 = t2.
+Lemma sub_lolli_inv A1 A2 s1 s2 B1 B2 :
+  Lolli A1 B1 s1 <: Lolli A2 B2 s2 -> 
+  A1 === A2 /\ B1 <: B2 /\ s1 = s2.
 Proof.
   move=> [A' B' []].
   - move=> C c1 c2. 
-    have{c1 c2}/lolli_inj[c1 [c2 [->->]]]: 
-      Lolli A1 B1 s1 t1 === Lolli A2 B2 s2 t2.
+    have{c1 c2}/lolli_inj[c1 [c2 ->]]: 
+      Lolli A1 B1 s1 === Lolli A2 B2 s2.
      exact: conv_trans c2.
     firstorder=>//. exact: conv_sub.
   - move=> *. exfalso; solve_conv.
   - move=> *. exfalso; solve_conv.
   - move=> *. exfalso; solve_conv.
-  - move=> A B0 B3 s t sb /lolli_inj[c1 [c2 [<-<-]]]. 
-    move=> /lolli_inj[c3 [c4 [->->]]]. 
+  - move=> A B0 B3 s sb /lolli_inj[c1 [c2 <-]]. 
+    move=> /lolli_inj[c3 [c4 ->]]. 
     firstorder.
     exact: conv_trans c3. exact: SubI sb c2 c4.
 Qed.
@@ -1104,94 +1102,94 @@ Proof. move=> *; by apply: sub_subst. Qed.
 
 Notation 𝐏 := (Sort U None).
 Reserved Notation "[ Γ |- ]".
-Reserved Notation "[ Γ |- m :- A -: s ]".
+Reserved Notation "[ Γ |- m :- A ]".
   
-Inductive has_type : context term -> term -> term -> sort -> Prop :=
+Inductive has_type : context term -> term -> term -> Prop :=
 | p_axiom Γ : 
   [ Γ ] ->
-  [ Γ |- 𝐏 :- U @ 0 -: U ]
+  [ Γ |- 𝐏 :- U @ 0 ]
 | s_axiom Γ s l : 
   [ Γ ] ->
-  [ Γ |- s @ l :- U @ l.+1 -: U ]
+  [ Γ |- s @ l :- U @ l.+1 ]
 | prop Γ A B l :
   [ Γ ] ->
-  [ Γ |- A :- Sort U l -: U ] ->
-  [ A +u Γ |- B :- 𝐏 -: U ] ->
-  [ Γ |- Prod A B U U :- 𝐏 -: U ]
+  [ Γ |- A :- Sort U l ] ->
+  [ A +u Γ |- B :- 𝐏 ] ->
+  [ Γ |- Prod A B U :- 𝐏 ]
 | u_prod Γ A B s l :
   [ Γ ] ->
-  [ Γ |- A :- U @ l -: U ] ->
-  [ A +u Γ |- B :- s @ l -: U ] ->
-  [ Γ |- Prod A B U s :- U @ l -: U ]
+  [ Γ |- A :- U @ l ] ->
+  [ A +u Γ |- B :- s @ l ] ->
+  [ Γ |- Prod A B U :- U @ l ]
 | l_prod Γ A B s l :
   [ Γ ] ->
-  [ Γ |- A :- L @ l -: U ] ->
-  [ □ Γ |- B :- s @ l -: U ] ->
-  [ Γ |- Prod A B L s :- U @ l -: U ]
+  [ Γ |- A :- L @ l ] ->
+  [ □ Γ |- B :- s @ l ] ->
+  [ Γ |- Prod A B L :- U @ l ]
 | u_lolli Γ A B s l :
   [ Γ ] ->
-  [ Γ |- A :- U @ l -: U ] ->
-  [ A +u Γ |- B :- s @ l -: U ] ->
-  [ Γ |- Lolli A B U s :- L @ l -: U ]
+  [ Γ |- A :- U @ l ] ->
+  [ A +u Γ |- B :- s @ l ] ->
+  [ Γ |- Lolli A B U :- L @ l ]
 | l_lolli Γ A B s l :
   [ Γ ] ->
-  [ Γ |- A :- L @ l -: U ] ->
-  [ □ Γ |- B :- s @ l -: U ] ->
-  [ Γ |- Lolli A B L s :- L @ l -: U ]
+  [ Γ |- A :- L @ l ] ->
+  [ □ Γ |- B :- s @ l ] ->
+  [ Γ |- Lolli A B L :- L @ l ]
 | u_var Γ x A : 
   [ x :u A ∈ Γ ] ->
-  [ Γ |- Var x :- A -: U ]
+  [ Γ |- Var x :- A ]
 | l_var Γ x A :
   [ x :l A ∈ Γ ] ->
-  [ Γ |- Var x :- A -: L ]
-| prod_lam Γ n A s B t l :
+  [ Γ |- Var x :- A ]
+| prod_lam Γ n A B s t l :
   [ Γ ] ->
-  [ Γ |- Prod A B s t :- Sort U l -: U ] ->
-  [ A +{s} Γ |- n :- B -: t ] ->
-  [ Γ |- Lam n :- Prod A B s t -: U ]
-| lolli_lam Γ n A s B t l :
-  [ %Γ |- Lolli A B s t :- L @ l -: U ] ->
-  [ A +{s} Γ |- n :- B -: t ] ->
-  [ Γ |- Lam n :- Lolli A B s t -: L ]
-| u_prod_app Γ₁ Γ₂ Γ A B s m n :
+  [ Γ |- Prod A B s :- Sort t l ] ->
+  [ A +{s} Γ |- n :- B ] ->
+  [ Γ |- Lam n :- Prod A B s ]
+| lolli_lam Γ n A B s t l :
+  [ %Γ |- Lolli A B s :- Sort t l ] ->
+  [ A +{s} Γ |- n :- B ] ->
+  [ Γ |- Lam n :- Lolli A B s ]
+| u_prod_app Γ₁ Γ₂ Γ A B m n :
   [ Γ₂ ] ->
-  [ Γ₁ |- m :- Prod A B U s -: U ] ->
-  [ Γ₂ |- n :- A -: U ] ->
+  [ Γ₁ |- m :- Prod A B U ] ->
+  [ Γ₂ |- n :- A ] ->
   [ Γ₁ ‡ Γ₂ ‡ Γ ] ->
-  [ Γ |- App m n :- B.[n/] -: s ]
-| l_prod_app Γ₁ Γ₂ Γ  A B s m n :
-  [ Γ₁ |- m :- Prod A B L s -: U ] ->
-  [ Γ₂ |- n :- A -: L ] ->
+  [ Γ |- App m n :- B.[n/] ]
+| l_prod_app Γ₁ Γ₂ Γ  A B m n :
+  [ Γ₁ |- m :- Prod A B L ] ->
+  [ Γ₂ |- n :- A ] ->
   [ Γ₁ ‡ Γ₂ ‡ Γ ] ->
-  [ Γ |- App m n :- B.[n/] -: s ]
-| u_lolli_app Γ₁ Γ₂ Γ A B s m n :
+  [ Γ |- App m n :- B.[n/] ]
+| u_lolli_app Γ₁ Γ₂ Γ A B m n :
   [ Γ₂ ] ->
-  [ Γ₁ |- m :- Lolli A B U s -: L ] ->
-  [ Γ₂ |- n :- A -: U ] ->
+  [ Γ₁ |- m :- Lolli A B U ] ->
+  [ Γ₂ |- n :- A ] ->
   [ Γ₁ ‡ Γ₂ ‡ Γ ] ->
-  [ Γ |- App m n :- B.[n/] -: s ]
-| l_lolli_app Γ₁ Γ₂ Γ  A B s m n :
-  [ Γ₁ |- m :- Lolli A B L s -: L ] ->
-  [ Γ₂ |- n :- A -: L ] ->
+  [ Γ |- App m n :- B.[n/] ]
+| l_lolli_app Γ₁ Γ₂ Γ  A B m n :
+  [ Γ₁ |- m :- Lolli A B L ] ->
+  [ Γ₂ |- n :- A ] ->
   [ Γ₁ ‡ Γ₂ ‡ Γ ] ->
-  [ Γ |- App m n :- B.[n/] -: s ]
+  [ Γ |- App m n :- B.[n/] ]
 | conversion Γ A B m s l :
   A <: B ->
-  [ %Γ |- B :- Sort s l -: U ] ->
-  [ Γ |- m :- A -: s ] ->
-  [ Γ |- m :- B -: s ]
-where "[ Γ |- m :- A -: s ]" := (has_type Γ m A s).
+  [ %Γ |- B :- Sort s l ] ->
+  [ Γ |- m :- A ] ->
+  [ Γ |- m :- B ]
+where "[ Γ |- m :- A ]" := (has_type Γ m A).
 
 Inductive context_ok : context term -> Prop :=
 | nil_ok :
   [ nil |- ]
 | u_ok Γ A l :
   [ Γ |- ] ->
-  [ %Γ |- A :- Sort U l -: U ] ->
+  [ %Γ |- A :- Sort U l ] ->
   [ A +u Γ |- ]
 | l_ok Γ A l :
   [ Γ |- ] ->
-  [ %Γ |- A :- Sort L l -: U ] ->
+  [ %Γ |- A :- Sort L l ] ->
   [ A +l Γ |- ]
 | n_ok Γ :
   [ Γ |- ] ->
@@ -1394,11 +1392,11 @@ Proof.
     repeat constructor; eauto.
 Qed.
 
-Lemma rename_ok Γ m A s :
-  [ Γ |- m :- A -: s ] ->
+Lemma rename_ok Γ m A :
+  [ Γ |- m :- A ] ->
   forall Γ' ξ,
     agree_ren ξ Γ Γ' ->
-    [ Γ' |- m.[ren ξ] :- A.[ren ξ] -: s ].
+    [ Γ' |- m.[ren ξ] :- A.[ren ξ] ].
 Proof.
   intros H.
   induction H; simpl; intros.
@@ -1414,25 +1412,25 @@ Proof.
     constructor; eauto.
   - asimpl.
     pose proof (agree_ren_pure H2 H).
-    apply u_prod; eauto.
+    eapply u_prod; eauto.
     replace (s @ l) with ((s @ l).[ren (upren ξ)]) by autosubst.
     apply IHhas_type2.
     constructor; eauto.
   - asimpl.
     pose proof (agree_ren_pure H2 H).
-    apply l_prod; eauto.
+    eapply l_prod; eauto.
     replace (s @ l) with ((s @ l).[ren (upren ξ)]) by autosubst.
     apply IHhas_type2.
     constructor; eauto.
   - asimpl.
     pose proof (agree_ren_pure H2 H).
-    apply u_lolli; eauto.
+    eapply u_lolli; eauto.
     replace (s @ l) with ((s @ l).[ren (upren ξ)]) by autosubst.
     apply IHhas_type2.
     constructor; eauto.
   - asimpl.
     pose proof (agree_ren_pure H2 H).
-    apply l_lolli; eauto.
+    eapply l_lolli; eauto.
     replace (s @ l) with ((s @ l).[ren (upren ξ)]) by autosubst.
     apply IHhas_type2.
     constructor; eauto.
@@ -1491,7 +1489,7 @@ Lemma hasU_ok Γ :
   [ Γ |- ] ->
   forall x A,
     [ x :u A ∈ Γ ] ->
-    exists l, [ %Γ |- A :- Sort U l -: U ].
+    exists l, [ %Γ |- A :- Sort U l ].
 Proof.
   induction 1; intros.
   - inv H.
@@ -1525,7 +1523,7 @@ Lemma hasL_ok Γ :
   [ Γ |- ] ->
   forall x A,
     [ x :l A ∈ Γ ] ->
-    exists l, [ %Γ |- A :- Sort L l -: U ].
+    exists l, [ %Γ |- A :- Sort L l ].
 Proof.
   induction 1; intros.
   - inv H.
@@ -1553,9 +1551,9 @@ Proof.
     apply agree_ren_refl.
 Qed.
 
-Lemma weakeningU Γ m A s B :
-  [ Γ |- m :- A -: s ] ->
-  [ B +u Γ |- m.[ren (+1)] :- A.[ren (+1)] -: s ].
+Lemma weakeningU Γ m A B :
+  [ Γ |- m :- A ] ->
+  [ B +u Γ |- m.[ren (+1)] :- A.[ren (+1)] ].
 Proof.
   intros.
   eapply rename_ok in H.
@@ -1564,9 +1562,9 @@ Proof.
   apply agree_ren_refl.
 Qed.
 
-Lemma weakeningN Γ m A s :
-  [ Γ |- m :- A -: s ] ->
-  [ □ Γ |- m.[ren (+1)] :- A.[ren (+1)] -: s ].
+Lemma weakeningN Γ m A :
+  [ Γ |- m :- A ] ->
+  [ □ Γ |- m.[ren (+1)] :- A.[ren (+1)] ].
 Proof.
   intros.
   eapply rename_ok in H.
@@ -1575,21 +1573,21 @@ Proof.
   apply agree_ren_refl.
 Qed.
 
-Lemma eweakeningU Γ m m' A A' s B :
+Lemma eweakeningU Γ m m' A A' B :
   m' = m.[ren (+1)] -> 
   A' = A.[ren (+1)] ->
-  [ Γ |- m :- A -: s ] -> 
-  [ B +u Γ |- m' :- A' -: s ].
+  [ Γ |- m :- A ] -> 
+  [ B +u Γ |- m' :- A' ].
 Proof.  
   intros; subst.
   apply weakeningU; eauto.
 Qed.
 
-Lemma eweakeningN Γ m m' A A' s :
+Lemma eweakeningN Γ m m' A A' :
   m' = m.[ren (+1)] -> 
   A' = A.[ren (+1)] ->
-  [ Γ |- m :- A -: s ] -> 
-  [ □ Γ |-m' :- A' -: s ].
+  [ Γ |- m :- A ] -> 
+  [ □ Γ |-m' :- A' ].
 Proof.  
   intros; subst.
   apply weakeningN; eauto.
@@ -1612,25 +1610,25 @@ Inductive agree_subst :
   [ □ Δ |- up σ -| □ Γ ]
 | agree_subst_wkU Δ σ Γ n A :
   [ Δ |- σ -| Γ ] ->
-  [ %Δ |- n :- A.[σ] -: U ] ->
+  [ %Δ |- n :- A.[σ] ] ->
   [ Δ |- n .: σ -| A +u Γ ]
 | agree_subst_wkL Δ₁ Δ₂ Δ σ Γ n A :
   merge Δ₁ Δ₂ Δ ->
   [ Δ₁ |- σ -| Γ ] ->
-  [ Δ₂ |- n :- A.[σ] -: L ] ->
+  [ Δ₂ |- n :- A.[σ] ] ->
   [ Δ |- n .: σ -| A +l Γ ]
 | agree_subst_wkN Δ σ Γ n :
   [ Δ |- σ -| Γ ] ->
   [ Δ |- n .: σ -| □ Γ ]
 | agree_subst_convU Δ σ Γ A B l :
   A <: B ->
-  [ %Δ |- B.[ren (+1)].[σ] :- Sort U l -: U ] ->
+  [ %Δ |- B.[ren (+1)].[σ] :- Sort U l ] ->
   [ Δ |- σ -| A +u Γ ] ->
   [ Δ |- σ -| B +u Γ ]
 | agree_subst_convL Δ σ Γ A B l :
   A <: B ->
-  [ %Δ |- B.[ren (+1)].[σ] :- Sort L l -: U ] ->
-  [ %Γ |- B :- Sort L l -: U ] ->
+  [ %Δ |- B.[ren (+1)].[σ] :- Sort L l ] ->
+  [ %Γ |- B :- Sort L l ] ->
   [ Δ |- σ -| A +l Γ ] ->
   [ Δ |- σ -| B +l Γ ]
 where "[ Δ |- σ -| Γ ]" := (agree_subst Δ σ Γ).
@@ -1677,7 +1675,7 @@ Lemma agree_subst_hasU Δ σ Γ :
   [ Δ |- σ -| Γ ] ->
   forall x A,
     [ x :u A ∈ Γ ] -> 
-    [ Δ |- σ x :- A.[σ] -: U ].
+    [ Δ |- σ x :- A.[σ] ].
 Proof.
   induction 1; intros.
   - inv H.
@@ -1715,7 +1713,7 @@ Lemma agree_subst_hasL Δ σ Γ :
   [ Δ |- σ -| Γ ] ->
   forall x A,
     [ x :l A ∈ Γ ] -> 
-    [ Δ |- σ x :- A.[σ] -: L ].
+    [ Δ |- σ x :- A.[σ] ].
 Proof.
   induction 1; intros.
   - inv H.
@@ -1725,7 +1723,7 @@ Proof.
     asimpl.
     replace (A.[σ >> ren (+1)]) 
       with (A.[σ].[ren (+1)]) by autosubst.
-    constructor.
+    apply l_var.
     constructor.
     eapply agree_subst_pure; eauto.
   - inv H0.
@@ -1888,11 +1886,11 @@ Proof.
       rewrite H12; eauto.
 Qed.
 
-Lemma substitution Γ m A s :
-  [ Γ |- m :- A -: s ] ->
+Lemma substitution Γ m A :
+  [ Γ |- m :- A ] ->
   forall Δ σ,
     [ Δ |- σ -| Γ ] ->
-    [ Δ |- m.[σ] :- A.[σ] -: s ].
+    [ Δ |- m.[σ] :- A.[σ] ].
 Proof.
   intros H.
   dependent induction H; asimpl; intros; eauto.
@@ -1908,22 +1906,22 @@ Proof.
   - specialize (IHhas_type1 _ _ H2). asimpl in IHhas_type1.
     pose proof (agree_subst_u A H2).
     specialize (IHhas_type2 _ _ H3).
-    apply u_prod; simpl; eauto.
+    eapply u_prod; simpl; eauto.
     eapply agree_subst_pure; eauto.
   - specialize (IHhas_type1 _ _ H2). asimpl in IHhas_type1.
     pose proof (agree_subst_n H2).
     specialize (IHhas_type2 _ _ H3).
-    apply l_prod; simpl; eauto.
+    eapply l_prod; simpl; eauto.
     eapply agree_subst_pure; eauto.
   - specialize (IHhas_type1 _ _ H2). asimpl in IHhas_type1.
     pose proof (agree_subst_u A H2).
     specialize (IHhas_type2 _ _ H3).
-    apply u_lolli; simpl; eauto.
+    eapply u_lolli; simpl; eauto.
     eapply agree_subst_pure; eauto.
   - specialize (IHhas_type1 _ _ H2). asimpl in IHhas_type1.
     pose proof (agree_subst_n H2).
     specialize (IHhas_type2 _ _ H3).
-    apply l_lolli; simpl; eauto.
+    eapply l_lolli; simpl; eauto.
     eapply agree_subst_pure; eauto.
   - eapply agree_subst_hasU; eauto.
   - eapply agree_subst_hasL; eauto.
@@ -1975,13 +1973,13 @@ Proof.
     apply IHhas_type2; eauto.
 Qed.
 
-Lemma substitutionU Γ₁ m A B s :
-  [ A +u Γ₁ |- m :- B -: s ] ->
+Lemma substitutionU Γ₁ m A B :
+  [ A +u Γ₁ |- m :- B ] ->
   forall Γ₂ Γ n,
     [ Γ₂ ] ->
     [ Γ₁ ‡ Γ₂ ‡ Γ ] -> 
-    [ Γ₂ |- n :- A -: U ] -> 
-    [ Γ |- m.[n/] :- B.[n/] -: s ].
+    [ Γ₂ |- n :- A ] -> 
+    [ Γ |- m.[n/] :- B.[n/] ].
 Proof.
   intros.
   eapply substitution.
@@ -1998,11 +1996,11 @@ Proof.
   rewrite <- pure_re; eauto.
 Qed.
 
-Lemma substitutionN Γ₁ m A B s :
-  [ □ Γ₁ |- m :- B -: s ] ->
-  forall Γ₂ n t,
-    [ Γ₂ |- n :- A -: t ] -> 
-    [ Γ₁ |- m.[n/] :- B.[n/] -: s ].
+Lemma substitutionN Γ₁ m A B :
+  [ □ Γ₁ |- m :- B ] ->
+  forall Γ₂ n,
+    [ Γ₂ |- n :- A ] -> 
+    [ Γ₁ |- m.[n/] :- B.[n/] ].
 Proof.
   intros.
   eapply substitution.
@@ -2011,12 +2009,12 @@ Proof.
   apply agree_subst_refl.
 Qed.
 
-Lemma substitutionL Γ₁ m A B s :
-  [ A +l Γ₁ |- m :- B -: s ] ->
+Lemma substitutionL Γ₁ m A B :
+  [ A +l Γ₁ |- m :- B ] ->
   forall Γ₂ Γ n,
     [ Γ₁ ‡ Γ₂ ‡ Γ ] -> 
-    [ Γ₂ |- n :- A -: L ] -> 
-    [ Γ |- m.[n/] :- B.[n/] -: s ].
+    [ Γ₂ |- n :- A ] -> 
+    [ Γ |- m.[n/] :- B.[n/] ].
 Proof.
   intros.
   eapply substitution.
@@ -2025,14 +2023,14 @@ Proof.
   apply agree_subst_refl.
 Qed.
 
-Lemma context_convU Γ m A B C s l :
+Lemma context_convU Γ m A B C l :
   B === A -> 
-  [ %Γ |- A :- Sort U l -: U ] ->
-  [ A +u Γ |- m :- C -: s ] -> 
-  [ B +u Γ |- m :- C -: s ].
+  [ %Γ |- A :- Sort U l ] ->
+  [ A +u Γ |- m :- C ] -> 
+  [ B +u Γ |- m :- C ].
 Proof.
   move=> conv tp1 tp2. 
-  cut ([ B +u Γ |- m.[ids] :- C.[ids] -: s ]). autosubst.
+  cut ([ B +u Γ |- m.[ids] :- C.[ids] ]). autosubst.
   eapply substitution.
   apply tp2.
   eapply agree_subst_convU; simpl.
@@ -2044,14 +2042,14 @@ Proof.
   apply agree_subst_refl.
 Qed.
 
-Lemma context_convL Γ m A B C s l :
+Lemma context_convL Γ m A B C l :
   B === A -> 
-  [ %Γ |- A :- Sort L l -: U ] ->
-  [ A +l Γ |- m :- C -: s ] -> 
-  [ B +l Γ |- m :- C -: s ].
+  [ %Γ |- A :- Sort L l ] ->
+  [ A +l Γ |- m :- C ] -> 
+  [ B +l Γ |- m :- C ].
 Proof.
   move=> conv tp1 tp2. 
-  cut ([ B +l Γ |- m.[ids] :- C.[ids] -: s ]). autosubst.
+  cut ([ B +l Γ |- m.[ids] :- C.[ids] ]). autosubst.
   eapply substitution.
   apply tp2.
   eapply agree_subst_convL; simpl.
@@ -2083,62 +2081,63 @@ Ltac solve_sub :=
   | _ => solve_conv
   end.
 
-Lemma u_prod_inv Γ A B s t :
-  [ %Γ |- Prod A B U s :- t -: U ] -> 
-  exists l,
-    [ %Γ |- A :- Sort U l -: U ] /\ 
-    [ A +u %Γ |- B :- Sort s l -: U ].
+Lemma u_prod_inv Γ A B s :
+  [ Γ |- Prod A B U :- s ] -> 
+  exists s l,
+    [ Γ |- A :- Sort U l ] /\ [ A +u Γ |- B :- Sort s l ].
 Proof.
-  move e:(Prod A B U s) => n tp. elim: tp A B s e => //{Γ n}.
-  move=> Γ A B l0 p tp1 _ tp2 _ A0 B0 s0 [->->->].
+  move e:(Prod A B U) => n tp. elim: tp A B e => //{Γ n s}.
+  move=> Γ A B l0 p tp1 _ tp2 _ A0 B0 [->->].
+    exists U.
     exists l0; firstorder.
     destruct l0; eauto.
     assert (𝐏 <: U @ n).
     apply sub_prop.
     eapply conversion; eauto.
     constructor; apply re_pure.
-  move=> Γ A B s l0 p tp1 ih1 tp2 ih2 A0 B0 s0 [->->->].
+  move=> Γ A B s l0 p tp1 ih1 tp2 ih2 A0 B0 [->->].
+    exists s.
     exists (Some l0); firstorder.
 Qed.
 
-Lemma l_prod_inv Γ A B s t :
-  [ %Γ |- Prod A B L s :- t -: U ] -> 
-  exists l,
-    [ %Γ |- A :- Sort L l -: U ] /\ 
-    [ □ %Γ |- B :- Sort s l -: U ].
+Lemma l_prod_inv Γ A B s :
+  [ Γ |- Prod A B L :- s ] -> 
+  exists s l,
+    [ Γ |- A :- Sort L l ] /\ [ □ Γ |- B :- Sort s l ].
 Proof.
-  move e:(Prod A B L s) => n tp. elim: tp A B s e => //{Γ n}.
-  move=> Γ A B s l0 p tp1 ih1 tp2 ih2 A0 B0 s0 [->->->].
+  move e:(Prod A B L) => n tp. elim: tp A B e => //{Γ n s}.
+  move=> Γ A B s l0 p tp1 ih1 tp2 ih2 A0 B0 [->->].
+    exists s.
     exists (Some l0); firstorder.
 Qed.
 
-Lemma u_lolli_inv Γ A B s t :
-  [ %Γ |- Lolli A B U s :- t -: U ] -> 
-  exists l,
-    [ %Γ |- A :- Sort U l -: U ] /\ 
-    [ A +u %Γ |- B :- Sort s l -: U ].
+Lemma u_lolli_inv Γ A B s :
+  [ Γ |- Lolli A B U :- s ] -> 
+  exists s l,
+    [ Γ |- A :- Sort U l ] /\ [ A +u Γ |- B :- Sort s l ].
 Proof.
-  move e:(Lolli A B U s) => n tp. elim: tp A B s e => //{Γ n}.
-  move=> Γ A B s l0 p tp1 ih1 tp2 ih2 A0 B0 s0 [->->->].
+  move e:(Lolli A B U) => n tp. elim: tp A B e => //{Γ n s}.
+  move=> Γ A B s l0 p tp1 ih1 tp2 ih2 A0 B0 [->->].
+    exists s.
     exists (Some l0); firstorder.
 Qed.
 
-Lemma l_lolli_inv Γ A B s t :
-  [ %Γ |- Lolli A B L s :- t -: U ] -> 
-  exists l,
-    [ %Γ |- A :- Sort L l -: U ] /\ 
-    [ □ %Γ |- B :- Sort s l -: U ].
+Lemma l_lolli_inv Γ A B s :
+  [ Γ |- Lolli A B L :- s ] -> 
+  exists s l,
+    [ Γ |- A :- Sort L l ] /\ [ □ Γ |- B :- Sort s l ].
 Proof.
-  move e:(Lolli A B L s) => n tp. elim: tp A B s e => //{Γ n}.
-  move=> Γ A B s l0 p tp1 ih1 tp2 ih2 A0 B0 s0 [->->->].
+  move e:(Lolli A B L) => n tp. elim: tp A B e => //{Γ n s}.
+  move=> Γ A B s l0 p tp1 ih1 tp2 ih2 A0 B0 [->->].
+    exists s.
     exists (Some l0); firstorder.
 Qed.
 
-Lemma prod_lam_invX Γ n C srt :
-  [ Γ |- Lam n :- C -: srt ] -> 
+Lemma prod_lam_invX Γ n C :
+  [ Γ |- Lam n :- C ] -> 
   forall A B s t l, 
-    (C <: Prod A B s t /\ [ %(A +{s} Γ) |- B :- Sort t l -: U]) ->
-    [ A +{s} Γ |- n :- B -: t ].
+    (C <: Prod A B s /\ [ %(A +{s} Γ) |- B :- Sort t l ]) ->
+    [ A +{s} Γ |- n :- B ].
 Proof.
   intros.
   dependent induction H; firstorder.
@@ -2147,17 +2146,17 @@ Proof.
     pose proof (pure_re H).
     rewrite H6 in H0.
     destruct s0.
-    + apply u_prod_inv in H0. inv H0.
+    + apply u_prod_inv in H0; first_order.
       eapply conversion; eauto.
       eapply context_convU.
       apply conv_sym; apply H4.
-      apply H7.
+      apply H0.
       apply H1.
-    + apply l_prod_inv in H0. inv H0.
+    + apply l_prod_inv in H0; first_order.
       eapply conversion; eauto.
       eapply context_convL.
       apply conv_sym; apply H4.
-      apply H7.
+      apply H0.
       apply H1.
   - exfalso; solve_sub.
   - eapply IHhas_type2; eauto.
@@ -2166,11 +2165,11 @@ Proof.
     apply H3.
 Qed.
 
-Lemma lolli_lam_invX Γ n C srt :
-  [ Γ |- Lam n :- C -: srt ] -> 
+Lemma lolli_lam_invX Γ n C :
+  [ Γ |- Lam n :- C ] -> 
   forall A B s t l, 
-    (C <: Lolli A B s t /\ [ %(A +{s} Γ) |- B :- Sort t l -: U]) ->
-    [ A +{s} Γ |- n :- B -: t ].
+    (C <: Lolli A B s /\ [ %(A +{s} Γ) |- B :- Sort t l ]) ->
+    [ A +{s} Γ |- n :- B ].
 Proof.
   intros.
   dependent induction H; firstorder.
@@ -2178,17 +2177,17 @@ Proof.
   - pose proof (sub_lolli_inv H1).
     first_order; subst.
     destruct s0.
-    + apply u_lolli_inv in H. inv H.
+    + apply u_lolli_inv in H; first_order.
       eapply conversion; eauto.
       eapply context_convU.
       apply conv_sym; apply H3.
-      apply H5.
+      apply H.
       apply H0.
-    + apply l_lolli_inv in H. inv H.
+    + apply l_lolli_inv in H; first_order.
       eapply conversion; eauto.
       eapply context_convL.
       apply conv_sym; apply H3.
-      apply H5.
+      apply H.
       apply H0.
   - eapply IHhas_type2; eauto.
     split.
@@ -2197,9 +2196,9 @@ Proof.
 Qed.
 
 Lemma prod_lam_inv Γ n A B s t l :
-  [ %Γ |- Prod A B s t :- Sort U l -: U ] ->
-  [ Γ |- Lam n :- Prod A B s t -: U ] -> 
-  [ A +{s} Γ |- n :- B -: t ].
+  [ %Γ |- Prod A B s :- Sort t l ] ->
+  [ Γ |- Lam n :- Prod A B s ] -> 
+  [ A +{s} Γ |- n :- B ].
 Proof.
   intros.
   destruct s.
@@ -2210,9 +2209,9 @@ Proof.
 Qed.
 
 Lemma lolli_lam_inv Γ n A B s t l :
-  [ %Γ |- Lolli A B s t :- Sort L l -: U ] ->
-  [ Γ |- Lam n :- Lolli A B s t -: L ] -> 
-  [ A +{s} Γ |- n :- B -: t ].
+  [ %Γ |- Lolli A B s:- Sort t l ] ->
+  [ Γ |- Lam n :- Lolli A B s ] -> 
+  [ A +{s} Γ |- n :- B ].
 Proof.
   intros.
   destruct s.
@@ -2257,47 +2256,78 @@ Proof.
     inv H2; split; constructor; eauto.
 Qed.
 
-Theorem propagation Γ m A s : 
+Theorem propagation Γ m A : 
   [ Γ |- ] ->
-  [ Γ |- m :- A -: s ] ->
-  exists l, [ %Γ |- A :- Sort s l -: U ].
+  [ Γ |- m :- A ] ->
+  exists s l, [ %Γ |- A :- Sort s l ].
 Proof.
   intros.
   dependent induction H0.
-  - exists (Some 1).
+  - exists U.
+    exists (Some 1).
     constructor.
     rewrite <- pure_re; eauto.
-  - exists (Some l.+2).
+  - exists U.
+    exists (Some l.+2).
     constructor.
     rewrite <- pure_re; eauto.
-  - exists (Some 0).
+  - exists U.
+    exists (Some 0).
     constructor.
     rewrite <- pure_re; eauto.
-  - exists (Some l.+1).
+  - exists U.
+    exists (Some l.+1).
     constructor.
     rewrite <- pure_re; eauto.
-  - exists (Some l.+1).
+  - exists U.
+    exists (Some l.+1).
     constructor.
     rewrite <- pure_re; eauto.
-  - exists (Some l.+1).
+  - exists U.
+    exists (Some l.+1).
     constructor.
     rewrite <- pure_re; eauto.
-  - exists (Some l.+1).
+  - exists U.
+    exists (Some l.+1).
     constructor.
     rewrite <- pure_re; eauto.
-  - eapply hasU_ok; eauto.
-  - eapply hasL_ok; eauto.
-  - exists l.
+  - exists U.
+    eapply hasU_ok; eauto.
+  - exists L.
+    eapply hasL_ok; eauto.
+  - exists t.
+    exists l.
     rewrite <- pure_re; eauto.
-  - exists (Some l); eauto.
+  - exists t.
+    exists l; eauto.
   - pose proof (merge_pure2 H1 H0).
     pose proof (merge_re_re H1). inv H3.
-    apply merge_context_ok_inv in H1; eauto. inv H1.
-    apply IHhas_type1 in H2. inv H2.
-    apply u_prod_inv in H1. first_order.
-    exists x0.
-    replace (Sort s x0) with ((Sort s x0).[n/]) by autosubst.
-    simpl in H7.
+    apply merge_context_ok_inv in H1; eauto. first_order.
+    apply u_prod_inv in H2. first_order.
+    exists x3.
+    exists x4.
+    replace (Sort x3 x4) with ((Sort x3 x4).[n/]) by autosubst.
+    eapply substitutionU; eauto.
+    replace (Γ₂) with (%Γ₁).
+    apply merge_re_re_re.
+    apply pure_re in H0.
+    rewrite H0.
+    rewrite H5; eauto.
+  - pose proof (merge_re_re H0). inv H1.
+    apply merge_context_ok_inv in H0; eauto. first_order.
+    eapply l_prod_inv in H5. first_order.
+    exists x3.
+    exists x4.
+    replace (Sort x3 x4) with ((Sort x3 x4).[n/]) by autosubst.
+    eapply substitutionN; eauto.
+    rewrite <- H2; eauto.
+  - pose proof (merge_pure2 H1 H0).
+    pose proof (merge_re_re H1). inv H3.
+    apply merge_context_ok_inv in H1; eauto. first_order.
+    apply u_lolli_inv in H2. first_order.
+    exists x3.
+    exists x4.
+    replace (Sort x3 x4) with ((Sort x3 x4).[n/]) by autosubst.
     eapply substitutionU; eauto.
     replace (Γ₂) with (re Γ₁).
     apply merge_re_re_re.
@@ -2305,68 +2335,45 @@ Proof.
     rewrite H0.
     rewrite H5; eauto.
   - pose proof (merge_re_re H0). inv H1.
-    apply merge_context_ok_inv in H0; eauto. inv H0.
-    apply IHhas_type1 in H1. inv H1.
-    eapply l_prod_inv in H0; eauto; inv H0.
-    exists x0.
-    replace (Sort s x0) with ((Sort s x0).[n/]) by autosubst.
+    apply merge_context_ok_inv in H0; eauto. first_order.
+    eapply l_lolli_inv in H5. first_order.
+    exists x3.
+    exists x4.
+    replace (Sort x3 x4) with ((Sort x3 x4).[n/]) by autosubst.
     eapply substitutionN; eauto.
-    rewrite <- H2.
-    apply H1.
-  - pose proof (merge_pure2 H1 H0).
-    pose proof (merge_re_re H1). inv H3.
-    apply merge_context_ok_inv in H1; eauto. inv H1.
-    apply IHhas_type1 in H2. inv H2.
-    apply u_lolli_inv in H1. first_order.
-    exists x0.
-    replace (Sort s x0) with ((Sort s x0).[n/]) by autosubst.
-    simpl in H7.
-    eapply substitutionU; eauto.
-    replace (Γ₂) with (re Γ₁).
-    apply merge_re_re_re.
-    apply pure_re in H0.
-    rewrite H0.
-    rewrite H5; eauto.
-  - pose proof (merge_re_re H0). inv H1.
-    apply merge_context_ok_inv in H0; eauto. inv H0.
-    apply IHhas_type1 in H1. inv H1.
-    eapply l_lolli_inv in H0; eauto; inv H0.
-    exists x0.
-    replace (Sort s x0) with ((Sort s x0).[n/]) by autosubst.
-    eapply substitutionN; eauto.
-    rewrite <- H2.
-    apply H1.
-  - exists l; eauto.
+    rewrite <- H2; eauto.
+  - exists s.
+    exists l; eauto.
 Qed.
 
 Lemma propL_false Γ A :
-  ~[ Γ |- Sort L None :- A -: U ].
+  ~[ Γ |- Sort L None :- A ].
 Proof.
   intro H.
   dependent induction H.
   apply IHhas_type2; eauto.
 Qed.
 
-Lemma has_propL_false Γ m s :
-  [ Γ |- ] -> [ Γ |- m :- Sort L None -: s ] -> False.
+Lemma has_propL_false Γ m :
+  [ Γ |- ] -> [ Γ |- m :- Sort L None ] -> False.
 Proof.
   intros.
-  apply propagation in H0; eauto.
-  inv H0.
-  apply propL_false in H1; eauto.
+  apply propagation in H0; eauto. 
+  first_order.
+  apply propL_false in H0; eauto.
 Qed.
 
-Theorem subject_reduction Γ m A s :
+Theorem subject_reduction Γ m A :
   [ Γ |- ] ->
-  [ Γ |- m :- A -: s ] ->
-  forall n, m ~> n -> [ Γ |- n :- A -: s ].
+  [ Γ |- m :- A ] ->
+  forall n, m ~> n -> [ Γ |- n :- A ].
 Proof.
   intros.
   dependent induction H0.
   - inv H1.
   - inv H1.
   - inv H1.
-    + specialize (IHhas_type1 H _ H7).
+    + specialize (IHhas_type1 H _ H6).
       eapply prop; eauto.
       eapply context_convU.
       eapply conv1i; eauto.
@@ -2375,10 +2382,10 @@ Proof.
     + assert ([A +u Γ |-]).
       eapply u_ok; eauto.
       rewrite <-pure_re; eauto.
-      specialize (IHhas_type2 H1 _ H7).
+      specialize (IHhas_type2 H1 _ H6).
       eapply prop; eauto.
   - inv H1.
-    + specialize (IHhas_type1 H _ H7).
+    + specialize (IHhas_type1 H _ H6).
       eapply u_prod; eauto.
       eapply context_convU.
       eapply conv1i; eauto.
@@ -2386,17 +2393,17 @@ Proof.
       eauto.
     + assert ([A +u Γ |-]).
       eapply u_ok; eauto; repeat rewrite <-pure_re; eauto.
-      specialize (IHhas_type2 H1 _ H7).
+      specialize (IHhas_type2 H1 _ H6).
       eapply u_prod; eauto.
   - inv H1.
-    + specialize (IHhas_type1 H _ H7).
+    + specialize (IHhas_type1 H _ H6).
       eapply l_prod; eauto.
     + assert ([□ Γ |-]).
       eapply n_ok; eauto.
-      specialize (IHhas_type2 H1 _ H7).
+      specialize (IHhas_type2 H1 _ H6).
       eapply l_prod; eauto.
   - inv H1.
-    + specialize (IHhas_type1 H _ H7).
+    + specialize (IHhas_type1 H _ H6).
       eapply u_lolli; eauto.
       eapply context_convU.
       eapply conv1i; eauto.
@@ -2404,14 +2411,14 @@ Proof.
       eauto.
     + assert ([A +u Γ |-]).
       eapply u_ok; eauto; repeat rewrite <-pure_re; eauto.
-      specialize (IHhas_type2 H1 _ H7).
+      specialize (IHhas_type2 H1 _ H6).
       eapply u_lolli; eauto.
   - inv H1.
-    + specialize (IHhas_type1 H _ H7).
+    + specialize (IHhas_type1 H _ H6).
       eapply l_lolli; eauto.
     + assert ([□ Γ |-]).
       eapply n_ok; eauto.
-      specialize (IHhas_type2 H1 _ H7).
+      specialize (IHhas_type2 H1 _ H6).
       eapply l_lolli; eauto.
   - inv H1.
   - inv H1.
@@ -2433,19 +2440,19 @@ Proof.
   - inv H1.
     pose proof H0_.
     destruct s.
-    + apply u_lolli_inv in H0_. first_order.
+    + apply u_lolli_inv in H0_; first_order.
       assert ([A +u Γ |-]).
       eapply u_ok; eauto.
       specialize (IHhas_type2 H4 _ H2).
       eapply lolli_lam; eauto.
-    + apply l_lolli_inv in H0_. first_order.
+    + apply l_lolli_inv in H0_; first_order.
       assert ([A +l Γ |-]).
       eapply l_ok; eauto.
       specialize (IHhas_type2 H4 _ H2).
       eapply lolli_lam; eauto.
   - pose proof (merge_context_ok_inv H1 H). inv H3.
     inv H2.
-    + pose proof (propagation H4 H0_). inv H2.
+    + pose proof (propagation H4 H0_); first_order.
       eapply substitutionU; eauto.
       eapply prod_lam_inv in H0_; eauto.
     + specialize (IHhas_type1 H4 _ H8).
@@ -2455,9 +2462,9 @@ Proof.
       apply conv_beta.
       apply conv1i; eauto.
       apply conv_sub in H2.
-      pose proof (propagation H4 H0_). inv H3.
-      apply u_prod_inv in H6; simpl in H6. first_order.
-      assert ([%Γ |- B.[n/] :- (Sort s x0).[n/] -: U ]).
+      pose proof (propagation H4 H0_); first_order.
+      apply u_prod_inv in H3; first_order.
+      assert ([%Γ |- B.[n/] :- (Sort x1 x2).[n/] ]).
       eapply substitutionU; eauto.
       pose proof (pure_re H0).
       pose proof (merge_re_re H1). inv H9.
@@ -2467,7 +2474,7 @@ Proof.
       eapply u_prod_app; eauto.
   - pose proof (merge_context_ok_inv H0 H). inv H2.
     inv H1.
-    + pose proof (propagation H3 H0_). inv H1.
+    + pose proof (propagation H3 H0_); first_order.
       eapply substitutionL; eauto.
       eapply prod_lam_inv in H0_; eauto.
     + specialize (IHhas_type1 H3 _ H7).
@@ -2477,9 +2484,9 @@ Proof.
       apply conv_beta.
       apply conv1i; eauto.
       apply conv_sub in H1.
-      pose proof (propagation H3 H0_). inv H2.
-      apply l_prod_inv in H5; simpl in H5. first_order.
-      assert ([%Γ |- B.[n/] :- (Sort s x0).[n/] -: U ]).
+      pose proof (propagation H3 H0_); first_order.
+      apply l_prod_inv in H2; first_order.
+      assert ([%Γ |- B.[n/] :- (Sort x1 x2).[n/] ]).
       eapply substitutionN; eauto.
       pose proof (merge_re_re H0). inv H6.
       rewrite <-H8; eauto.
@@ -2487,7 +2494,7 @@ Proof.
       eapply l_prod_app; eauto.
   - pose proof (merge_context_ok_inv H1 H). inv H3.
     inv H2.
-    + pose proof (propagation H4 H0_). inv H2.
+    + pose proof (propagation H4 H0_); first_order.
       eapply substitutionU; eauto.
       eapply lolli_lam_inv in H0_; eauto.
     + specialize (IHhas_type1 H4 _ H8).
@@ -2497,9 +2504,9 @@ Proof.
       apply conv_beta.
       apply conv1i; eauto.
       apply conv_sub in H2.
-      pose proof (propagation H4 H0_). inv H3.
-      apply u_lolli_inv in H6; simpl in H6. first_order.
-      assert ([%Γ |- B.[n/] :- (Sort s x0).[n/] -: U ]).
+      pose proof (propagation H4 H0_); first_order.
+      apply u_lolli_inv in H3; first_order.
+      assert ([%Γ |- B.[n/] :- (Sort x1 x2).[n/] ]).
       eapply substitutionU; eauto.
       pose proof (pure_re H0).
       pose proof (merge_re_re H1). inv H9.
@@ -2509,7 +2516,7 @@ Proof.
       eapply u_lolli_app; eauto.
   - pose proof (merge_context_ok_inv H0 H). inv H2.
     inv H1.
-    + pose proof (propagation H3 H0_). inv H1.
+    + pose proof (propagation H3 H0_); first_order.
       eapply substitutionL; eauto.
       eapply lolli_lam_inv in H0_; eauto.
     + specialize (IHhas_type1 H3 _ H7).
@@ -2519,9 +2526,9 @@ Proof.
       apply conv_beta.
       apply conv1i; eauto.
       apply conv_sub in H1.
-      pose proof (propagation H3 H0_). inv H2.
-      apply l_lolli_inv in H5; simpl in H5. first_order.
-      assert ([%Γ |- B.[n/] :- (Sort s x0).[n/] -: U ]).
+      pose proof (propagation H3 H0_); first_order.
+      apply l_lolli_inv in H2; first_order.
+      assert ([%Γ |- B.[n/] :- (Sort x1 x2).[n/] ]).
       eapply substitutionN; eauto.
       pose proof (merge_re_re H0). inv H6.
       rewrite <-H8; eauto.
@@ -2532,10 +2539,10 @@ Qed.
 
 Theorem subject_reduction_red m n :
   m ~>* n ->
-  forall Γ A s,
+  forall Γ A,
     [ Γ |- ] ->
-    [ Γ |- m :- A -: s ] ->
-    [ Γ |- n :- A -: s ].
+    [ Γ |- m :- A ] ->
+    [ Γ |- n :- A ].
 Proof.
   intro H.
   dependent induction H; intros; eauto.
@@ -2545,10 +2552,10 @@ Proof.
   apply H0.
 Qed.
 
-Lemma canonical_prod m C srt :
-  [ nil |- m :- C -: srt ] -> value m ->
-  forall A B s t, 
-    C <: Prod A B s t -> exists m', m = Lam m'.
+Lemma canonical_prod m C :
+  [ nil |- m :- C ] -> value m ->
+  forall A B s, 
+    C <: Prod A B s -> exists m', m = Lam m'.
 Proof.
   intros.
   dependent induction H; try (exfalso; solve_sub).
@@ -2559,10 +2566,10 @@ Proof.
     eapply sub_trans; eauto.
 Qed.
 
-Lemma canonical_lolli m C srt :
-  [ nil |- m :- C -: srt ] -> value m ->
-  forall A B s t, 
-    C <: Lolli A B s t -> exists m', m = Lam m'.
+Lemma canonical_lolli m C :
+  [ nil |- m :- C ] -> value m ->
+  forall A B s, 
+    C <: Lolli A B s -> exists m', m = Lam m'.
 Proof.
   intros.
   dependent induction H; try (exfalso; solve_sub).
@@ -2573,8 +2580,8 @@ Proof.
     eapply sub_trans; eauto.
 Qed.
 
-Theorem progress m A s :
-  [ nil |- m :- A -: s ] -> value m \/ exists n, step m n.
+Theorem progress m A :
+  [ nil |- m :- A ] -> value m \/ exists n, step m n.
 Proof.
   intros.
   dependent induction H; try solve [left; constructor].
@@ -2689,8 +2696,8 @@ Fixpoint occurs (i : nat) (m : term) : nat :=
   match m with
   | Var x => if x == i then 1 else 0
   | Sort _ _ => 0
-  | Prod A B _ _ => occurs i A + occurs (i.+1) B
-  | Lolli A B _ _ => occurs i A + occurs (i.+1) B
+  | Prod A B _ => occurs i A + occurs (i.+1) B
+  | Lolli A B _ => occurs i A + occurs (i.+1) B
   | Lam m => occurs (i.+1) m
   | App m n => occurs i m + occurs i n
   end.
@@ -2812,8 +2819,8 @@ Proof.
   - inv H0; firstorder; constructor; firstorder.
 Qed.
 
-Lemma narity Γ m A s :
-  [ Γ |- m :- A -: s ] -> 
+Lemma narity Γ m A :
+  [ Γ |- m :- A ] -> 
     forall i, [ i ∉ Γ ] -> occurs i m = 0.
 Proof.
   intro H.
@@ -2854,8 +2861,8 @@ Proof.
   - apply IHhas_type2; eauto.
 Qed.
 
-Theorem linearity Γ m A s :
-  [ Γ |- m :- A -: s ] -> 
+Theorem linearity Γ m A :
+  [ Γ |- m :- A ] -> 
     forall i, [ i ∈ Γ ] -> occurs i m = 1.
 Proof.
   intro H.
@@ -2934,8 +2941,8 @@ Fixpoint erase (m : CLC.term) : CC.term :=
   match m with
   | CLC.Var x => CC.Var x
   | CLC.Sort _ l => CC.Sort l
-  | CLC.Prod A B _ _ => CC.Prod (erase A) (erase B)
-  | CLC.Lolli A B _ _ => CC.Prod (erase A) (erase B)
+  | CLC.Prod A B _ => CC.Prod (erase A) (erase B)
+  | CLC.Lolli A B _ => CC.Prod (erase A) (erase B)
   | CLC.Lam n => CC.Lam (erase n)
   | CLC.App m n => CC.App (erase m) (erase n)
   end.
@@ -3203,9 +3210,9 @@ Proof.
   destruct x; simpl; eauto.
 Qed.
 
-Theorem embedding Γ m A s : 
-  [ Γ |- m :- A -: s ] ->
-  [ [[ Γ ]] |- [| m |] :- [| A |] ].
+Theorem embedding Γ m A : 
+  CLC.has_type Γ m A ->
+  CC.has_type [[ Γ ]] [| m |] [| A |].
 Proof.
   intro H.
   dependent induction H; asimpl.
@@ -3332,8 +3339,8 @@ Proof.
   econstructor; eauto.
 Qed.
 
-Theorem strong_normalization Γ m A s :
-  [ Γ |- m :- A -: s ] -> (sn CLC.step m).
+Theorem strong_normalization Γ m A :
+  CLC.has_type Γ m A -> (sn CLC.step m).
 Proof.
   intros.
   pose proof (embedding H).
